examples/Sek/PChunkImpl_proof.v
@@ -22,8 +22,8 @@ Require Import EChunkImpl_proof.
 
 
 (* Pourquoi je suis obligé de le remettre ?? *)
-Instance MonType_Memory A {IA: Inhab A} {EA: Enc A} :
-	MonType (Memory A) :=	make_MonType (Shared) (Extend).
+Instance MonType_PArrayMem A {IA: Inhab A} {EA: Enc A} :
+	MonType (PArrayMem A) :=	make_MonType (PArrayMemory) (PArrayExtend).
 
 Ltac xcf_pre tt ::=
 	intros; match goal with |- TripleMon _ _ _ _ => unfold TripleMon | _ => idtac end.
@@ -41,23 +41,23 @@ Record PChunkInv A {IA: Inhab A} (L: list A) (D: list A) (front: int) (size: int
 		pchunk_front : 0 <= front < K;
 		pchunk_size : 0 <= size <= K }.
 
-Definition IsPChunk A {IA: Inhab A} {EA: Enc A} (M: Memory A) (L: list A) (c: pchunk_ A) : Prop :=
+Definition IsPChunk A {IA: Inhab A} {EA: Enc A} (M: PArrayMem A) (L: list A) (c: pchunk_ A) : Prop :=
 	let (data, front, size, default) := c in
 	exists (D: list A),
 		IsPArray M D data /\
 		PChunkInv L D front size default.
 
-Lemma IsPChunk_inv_IsPArray : forall A (IA: Inhab A) (EA: Enc A) (M: Memory A) (c: pchunk_ A) (L: list A),
+Lemma IsPChunk_inv_IsPArray : forall A (IA: Inhab A) (EA: Enc A) (M: PArrayMem A) (c: pchunk_ A) (L: list A),
 	IsPChunk M L c ->
 	exists D, IsPArray M D (data' c).
 Proof. unfold IsPChunk. intros. destruct c. simpl. destruct~ H as [D [Rdata I]]. Qed.
 
-Lemma IsPChunk_inv_PChunkInv : forall A (IA: Inhab A) (EA: Enc A) (M: Memory A) (c: pchunk_ A) (L: list A),
+Lemma IsPChunk_inv_PChunkInv : forall A (IA: Inhab A) (EA: Enc A) (M: PArrayMem A) (c: pchunk_ A) (L: list A),
 	IsPChunk M L c ->
 	exists D, PChunkInv L D (front' c) (size' c) (default' c).
 Proof. unfold IsPChunk. intros. destruct c. simpl. destruct~ H as [D [Rdata I]]. Qed.
 
-Lemma IsPChunk_inv_length : forall A (IA: Inhab A) (EA: Enc A) (M: Memory A) (c: pchunk_ A) (L: list A),
+Lemma IsPChunk_inv_length : forall A (IA: Inhab A) (EA: Enc A) (M: PArrayMem A) (c: pchunk_ A) (L: list A),
 	IsPChunk M L c -> 0 <= length L <= K.
 Proof.
 	intros. forwards [D I]: IsPChunk_inv_PChunkInv H.
@@ -66,23 +66,23 @@ Qed.
 
 Hint Resolve IsPChunk_inv_IsPArray IsPChunk_inv_PChunkInv IsPChunk_inv_length.
 
-Definition IsHead A {IA: Inhab A} {EA: Enc A} (M: Memory A) (c: pchunk_ A) : hprop :=
+Definition IsHead A {IA: Inhab A} {EA: Enc A} (M: PArrayMem A) (c: pchunk_ A) : hprop :=
 	IsHead M (data' c).
 
-Definition access_cost A {IA: Inhab A} {EA: Enc A} (ishd: bool) (M: Memory A) (c: pchunk_ A) : hprop :=
+Definition access_cost A {IA: Inhab A} {EA: Enc A} (ishd: bool) (M: PArrayMem A) (c: pchunk_ A) : hprop :=
 	if ishd then IsHead M c \* \$1 else \$(2 * K + 2).
 
-Lemma access_cost_eq : forall A {IA: Inhab A} {EA: Enc A} (ishd: bool) (M: Memory A) (c: pchunk_ A) (L D: list A),
+Lemma access_cost_eq : forall A {IA: Inhab A} {EA: Enc A} (ishd: bool) (M: PArrayMem A) (c: pchunk_ A) (L D: list A),
 	IsPArray M D (data' c) ->
 		access_cost ishd M c =
 		parray_rebase_and_get_array_cost ishd M (data' c) D.
 Admitted.
 
-Lemma rebase_cost_true : forall A {IA: Inhab A} {EA: Enc A} (M: Memory A) (pa: PArray_ml.parray_ A) (L: list A),
+Lemma rebase_cost_true : forall A {IA: Inhab A} {EA: Enc A} (M: PArrayMem A) (pa: PArray_ml.parray_ A) (L: list A),
 	parray_rebase_and_get_array_cost true M pa L = PArray_proof.IsHead M pa \* \$1.
 Admitted.
 
-Lemma rebase_cost_false : forall A {IA: Inhab A} {EA: Enc A} (M: Memory A) (pa: PArray_ml.parray_ A) (L: list A),
+Lemma rebase_cost_false : forall A {IA: Inhab A} {EA: Enc A} (M: PArrayMem A) (pa: PArray_ml.parray_ A) (L: list A),
 	parray_rebase_and_get_array_cost false M pa L = \$(length L + bound L + 2).
 Admitted.
 
@@ -92,7 +92,7 @@ Hint Resolve access_cost_eq rebase_cost_true.
 (*************************************************)
 (** Specifications *)
 
-Lemma pchunk_default_spec : forall A (IA: Inhab A) (EA: Enc A) (M: Memory A) (L: list A) (c: pchunk_ A),
+Lemma pchunk_default_spec : forall A (IA: Inhab A) (EA: Enc A) (M: PArrayMem A) (L: list A) (c: pchunk_ A),
 	IsPChunk M L c ->
 	SPEC (pchunk_default c)
 		PRE (\$1)
@@ -101,13 +101,13 @@ Proof. unfolds IsPChunk. introv Rc. xcf. xpay. xvals~. Qed.
 
 Hint Extern 1 (RegisterSpec pchunk_default) => Provide pchunk_default_spec.
 
-Lemma pchunk_create_spec : forall A (IA: Inhab A) (EA: Enc A) (M: Memory A) (a: A),
+Lemma pchunk_create_spec : forall A (IA: Inhab A) (EA: Enc A) (M: PArrayMem A) (a: A),
 	SPEC (pchunk_create a)
 		MONO M
 		PRE (\$(K + 3))
 		POST (fun M' c => \[IsPChunk M' nil c] \* IsHead M' c).
 Proof.
-	xcf. xpay. xapp~ ;=> data M' HM' Rdata.
+	xcf. xpay. xapp~ ;=> data M' HM' Rdata _.
 	xvals~.
 	unfolds~ IsPChunk. exists (make K a). split~.
 	{ constructors~; intros.
@@ -118,7 +118,7 @@ Qed.
 
 Hint Extern 1 (RegisterSpec pchunk_create) => Provide pchunk_create_spec.
 
-Lemma pchunk_is_empty_spec : forall A (IA: Inhab A) (EA: Enc A) (M: Memory A) (L: list A) (c: pchunk_ A),
+Lemma pchunk_is_empty_spec : forall A (IA: Inhab A) (EA: Enc A) (M: PArrayMem A) (L: list A) (c: pchunk_ A),
 	IsPChunk M L c ->
 	SPEC (pchunk_is_empty c)
 		PRE (\$1)
@@ -131,7 +131,7 @@ Qed.
 
 Hint Extern 1 (RegisterSpec pchunk_is_empty) => Provide pchunk_is_empty_spec.
 
-Lemma pchunk_is_full_spec : forall A (IA: Inhab A) (EA: Enc A) (M: Memory A) (L: list A) (c: pchunk_ A),
+Lemma pchunk_is_full_spec : forall A (IA: Inhab A) (EA: Enc A) (M: PArrayMem A) (L: list A) (c: pchunk_ A),
 	IsPChunk M L c ->
 	SPEC (pchunk_is_full c)
 		PRE (\$1)
@@ -140,18 +140,18 @@ Admitted.
 
 Hint Extern 1 (RegisterSpec pchunk_is_full) => Provide pchunk_is_full_spec.
 
-Lemma pchunk_peek_back_spec : forall A (IA: Inhab A) (EA: Enc A) (ishd: bool) (M: Memory A) (L: list A) (c: pchunk_ A),
+Lemma pchunk_peek_back_spec : forall A (IA: Inhab A) (EA: Enc A) (ishd: bool) (M: PArrayMem A) (L: list A) (c: pchunk_ A),
 	IsPChunk M L c ->
 	L <> nil ->
 	SPEC (pchunk_peek_back c)
 		PRE (\$5 \* access_cost ishd M c)
-		INV (Shared M)
+		INV (PArrayMemory M)
 		POST (fun x => IsHead M c \* \exists L', \[L = L' & x]).
 Admitted.
 
 Hint Extern 1 (RegisterSpec pchunk_peek_back) => Provide pchunk_peek_back_spec.
 
-Lemma pchunk_pop_back_spec : forall A (IA: Inhab A) (EA: Enc A) (ishd: bool) (M: Memory A) (L: list A) (c: pchunk_ A),
+Lemma pchunk_pop_back_spec : forall A (IA: Inhab A) (EA: Enc A) (ishd: bool) (M: PArrayMem A) (L: list A) (c: pchunk_ A),
 	IsPChunk M L c ->
 	L <> nil -> 
 	SPEC (pchunk_pop_back c)
@@ -168,9 +168,9 @@ Proof.
 	unfold IsHead; simpl. rewrites~ (>> access_cost_eq D); simpl.
 	xapp~; simpl.
 	{ unwrap_up. }
-	{	intros x' M' E ->. xchange~ <- rebase_cost_true D. xapp~.
+	{	intros x' M' E -> _. xchange~ <- rebase_cost_true D. xapp~.
 		{ unwrap_up. }
-		{ intros pa M'' E' Rpa. xlets. xvals~.
+		{ intros pa M'' E' Rpa _. xlets. xvals~.
 			unfold IsPChunk. exists. split~.
 			{ constructors* ;=> i Hi.
 				{ applys_eq* Iin; list_cases*.
@@ -185,7 +185,7 @@ Qed.
 
 Hint Extern 1 (RegisterSpec pchunk_pop_back) => Provide pchunk_pop_back_spec.
 
-Lemma pchunk_push_back_spec : forall A (IA: Inhab A) (EA: Enc A) (ishd: bool) (M: Memory A) (c: pchunk_ A) (x: A) (L: list A),
+Lemma pchunk_push_back_spec : forall A (IA: Inhab A) (EA: Enc A) (ishd: bool) (M: PArrayMem A) (c: pchunk_ A) (x: A) (L: list A),
 	IsPChunk M L c ->
 	~ (IsFull L) ->
 	SPEC (pchunk_push_back c x)
@@ -197,24 +197,24 @@ Proof.
 	destruct c; simpls. lets~ [D [Rdata [Iin Iout Ilen Icapa Ifront Isz]]]: Rc.
 	xapp. rewrites~ (>> access_cost_eq L D); simpl. xapp~.
 	{ unwrap_up. }
-	{ intros pa M' E Rpa. xvals~. unfold IsPChunk. exists; split~.
+	{ intros pa M' E Rpa _. xvals~. unfold IsPChunk. exists; split~.
 		{ constructors* ;=> i Hi; list_cases*; unwrap_up in *; false; math. } }
 Qed.
 
 Hint Extern 1 (RegisterSpec pchunk_push_back) => Provide pchunk_push_back_spec.
 
-Lemma pchunk_peek_front_spec : forall A (IA: Inhab A) (EA: Enc A) (ishd: bool) (M: Memory A) (c: pchunk_ A) (L: list A),
+Lemma pchunk_peek_front_spec : forall A (IA: Inhab A) (EA: Enc A) (ishd: bool) (M: PArrayMem A) (c: pchunk_ A) (L: list A),
 	IsPChunk M L c ->
 	L <> nil ->
 	SPEC (pchunk_peek_front c)
 		PRE (\$5 \* access_cost ishd M c)
-		INV (Shared M)
+		INV (PArrayMemory M)
 		POST (fun x => IsHead M c \* \exists L', \[L = x :: L']).
 Admitted.
 
 Hint Extern 1 (RegisterSpec pchunk_peek_front) => Provide pchunk_peek_front_spec.
 
-Lemma pchunk_pop_front_spec : forall A (IA: Inhab A) (EA: Enc A) (ishd: bool) (M: Memory A) (c: pchunk_ A) (L: list A),
+Lemma pchunk_pop_front_spec : forall A (IA: Inhab A) (EA: Enc A) (ishd: bool) (M: PArrayMem A) (c: pchunk_ A) (L: list A),
 	IsPChunk M L c ->
 	L <> nil -> 
 	SPEC (pchunk_pop_front c)
@@ -228,7 +228,7 @@ Admitted.
 
 Hint Extern 1 (RegisterSpec pchunk_pop_front) => Provide pchunk_pop_front_spec.
 
-Lemma pchunk_push_front_spec : forall A (IA: Inhab A) (EA: Enc A) (ishd: bool) (M: Memory A) (c: pchunk_ A) (x: A) (L: list A),
+Lemma pchunk_push_front_spec : forall A (IA: Inhab A) (EA: Enc A) (ishd: bool) (M: PArrayMem A) (c: pchunk_ A) (x: A) (L: list A),
 	IsPChunk M L c ->
 	~ (IsFull L) ->
 	SPEC (pchunk_push_back c x)
@@ -239,18 +239,18 @@ Admitted.
 
 Hint Extern 1 (RegisterSpec pchunk_push_front) => Provide pchunk_push_front_spec.
 
-Lemma pchunk_get_spec : forall A (IA: Inhab A) (EA: Enc A) (ishd: bool) (M: Memory A) (c: pchunk_ A) (L: list A) (i: int),
+Lemma pchunk_get_spec : forall A (IA: Inhab A) (EA: Enc A) (ishd: bool) (M: PArrayMem A) (c: pchunk_ A) (L: list A) (i: int),
 	IsPChunk M L c ->
 	index L i ->
 	SPEC (pchunk_get c i)
 		PRE (\$4 \* access_cost ishd M c)
-		INV (Shared M)
+		INV (PArrayMemory M)
 		POST (fun x => IsHead M c \* \[x = L[i]]).
 Admitted.
 
 Hint Extern 1 (RegisterSpec pchunk_get) => Provide pchunk_get_spec.
 
-Lemma pchunk_set_spec : forall A (IA: Inhab A) (EA: Enc A) (ishd: bool) (M: Memory A) (c: pchunk_ A) (L: list A) (i: int) (x: A),
+Lemma pchunk_set_spec : forall A (IA: Inhab A) (EA: Enc A) (ishd: bool) (M: PArrayMem A) (c: pchunk_ A) (L: list A) (i: int) (x: A),
 	IsPChunk M L c ->
 	index L i ->
 	SPEC (pchunk_set c i x)
@@ -261,21 +261,21 @@ Proof.
 	introv Rc Hi. xcf; simpl. xpay. xapp.
 	destruct c; simpls. lets [D [Rdata [Iin Iout Ilen Icapa Ifront Isz]]]: Rc. xchange~ access_cost_eq; simpl. xapp~.
 	{ rew_index in *. unwrap_up. }
-	{ intros pa M' E Rpa. xvals~.
+	{ intros pa M' E Rpa _. xvals~.
 		unfold IsPChunk. exists; split~.
 		{ constructors* ;=> j Hj; list_cases*; unwrap_up in *; false; math. } }
 Qed.
 
 Hint Extern 1 (RegisterSpec pchunk_set) => Provide pchunk_set_spec.
 
-Lemma pchunk_of_echunk_spec : forall A (IA: Inhab A) (EA: Enc A) (M: Memory A) (ec: EChunkImpl_ml.echunk_ A) (L: list A),
+Lemma pchunk_of_echunk_spec : forall A (IA: Inhab A) (EA: Enc A) (M: PArrayMem A) (ec: EChunkImpl_ml.echunk_ A) (L: list A),
 	SPEC (pchunk_of_echunk ec)
 		MONO M
 		PRE (\$3 \* ec ~> EChunk L)
 		POST (fun M' pc => IsHead M' pc \* \[IsPChunk M' L pc]).
 Proof.
 	xcf*. xpay. xapp ;=> [[[data front] size] default]. xpull ;=> D I. xmatch.
-	xapp ;=> pa M' E Rpa. xvals~.
+	xapp ;=> pa M' E Rpa _. xvals~.
 	unfold IsPChunk. exists D. split~.
 	destruct I. constructors~.
 Qed.
